Vegas.lean
@@ -7,6 +7,7 @@ Authors: VegasCore contributors
 import GameTheory
 import Vegas.Core
 import Vegas.Source
+import Vegas.Graph
 import Vegas.Foundation.ViewExtension
 import Vegas.EventGraph
 import Vegas.Protocol
