Vegas/Graph.lean
@@ -1,0 +1,4 @@
+/- Copyright (c) 2026 VegasCore contributors. All rights reserved. -/
+
+import Vegas.Graph.Basic
+import Vegas.Graph.Semantics
